src/basic/RMWinstrProps.v
@@ -1,0 +1,205 @@
+Require Import RelationClasses List Lia.
+From PromisingLib Require Import Basic.
+From hahn Require Import Hahn.
+Require Import AuxDef.
+Require Import Events.
+Require Import Execution.
+Require Import Prog.
+Require Import ProgToExecution.
+Require Import ProgToExecutionProperties.
+
+Set Implicit Arguments.
+
+Section XACQ.
+
+Definition rmw_is_xacq_instr (i : Instr.t) :=
+  match i with
+  | Instr.update _ _ Xpln _ _  _ _ => False
+  | _ => True
+  end.
+
+Definition rmw_is_xacq_instrs (il : list Instr.t) :=
+  forall (i : Instr.t) (IN : In i il), rmw_is_xacq_instr i.
+
+Definition w_ex_is_xacq s :=
+  W_ex (ProgToExecution.G s) ⊆₁
+  W_ex (ProgToExecution.G s) ∩₁ is_xacq (lab (ProgToExecution.G s)).
+
+Lemma w_ex_is_xacq_add_preserves thread s s'
+      (WF : wf_thread_state thread s) lbl vl lc cl ff
+      (UG : G s' =
+            add (G s) thread (eindex s) lbl vl lc cl ff) 
+      (SS : w_ex_is_xacq s) :
+    w_ex_is_xacq s'.
+Proof.
+  unfold w_ex_is_xacq in *.
+  apply set_subset_inter_r. split; [done|].
+  unfold W_ex in *.
+  unfold add in UG. rewrite UG at 1. simpls.
+  rewrite SS. rewrite (dom_r WF.(wft_rmwE)).
+  rewrite codom_eqv1. rewrite set_interA.
+  unfolder. ins. desc.
+  unfold is_xacq, xmod. erewrite add_preserves_lab; eauto.
+Qed.
+
+Lemma w_ex_is_xacq_add_rmw_preserves thread s s'
+      (WF : wf_thread_state thread s) lbl1 ordw vl lc vl' lc' cl ff
+      (UG : G s' =
+            add_rmw (G s) thread (eindex s) lbl1
+                    (Astore Xacq ordw vl lc) vl' lc' cl ff) 
+      (SS : w_ex_is_xacq s) :
+    w_ex_is_xacq s'.
+Proof.
+  unfold w_ex_is_xacq in *.
+  apply set_subset_inter_r. split; [done|].
+  unfold W_ex in *.
+  unfold add_rmw in UG. rewrite UG at 1. simpls.
+  rewrite codom_union. unionL.
+  2: { rewrite SS. rewrite (dom_r WF.(wft_rmwE)).
+       rewrite codom_eqv1. rewrite set_interA.
+       unfolder. ins. desc.
+       unfold is_xacq, xmod. erewrite add_rmw_preserves_lab; eauto. }
+  subst. unfolder. ins. desf.
+  rewrite UG. simpls. unfold is_xacq, xmod. by rewrite upds.
+Qed.
+
+Lemma rmw_is_xacq_instr_xmod rmw rexmod xmod ordr ordw reg lexpr s
+      (XACQIN : rmw_is_xacq_instrs s.(instrs))
+      (ISTEP :
+         Some
+           (Instr.update rmw rexmod xmod ordr ordw reg
+                         lexpr) = nth_error (instrs s) (pc s)) :
+  xmod = Xacq.
+Proof.
+  symmetry in ISTEP; apply nth_error_In in ISTEP.
+  apply XACQIN in ISTEP; simpls; desf.
+Qed.
+
+Lemma w_ex_is_xacq_thread_step thread s s'
+      (XACQIN : rmw_is_xacq_instrs s.(instrs))
+      (WF : wf_thread_state thread s)
+      (STEP : step thread s s')
+      (SS : w_ex_is_xacq s) :
+  w_ex_is_xacq s'.
+Proof.
+  unfold w_ex_is_xacq in *.
+  destruct STEP as [ll STEP]. cdes STEP.
+  destruct ISTEP0.
+  1,2: by rewrite UG.
+  1-4: by eapply w_ex_is_xacq_add_preserves; eauto.
+  all: assert (xmod = Xacq); subst;
+    [ |eapply w_ex_is_xacq_add_rmw_preserves; eauto].
+  all: eapply rmw_is_xacq_instr_xmod; eauto.
+Qed.
+
+End XACQ.
+
+Section REX.
+
+Definition rmw_is_rex_instr (i : Instr.t) : Prop :=
+  match i with
+  | Instr.update _ false _ _ _ _ _ => False
+  | _ => True
+  end.
+
+Definition rmw_is_rex_instrs (il : list Instr.t) :=
+  forall (i : Instr.t) (IN : In i il), rmw_is_rex_instr i.
+
+Definition dom_rmw_in_rex s :=
+  dom_rel (rmw (ProgToExecution.G s)) ⊆₁ R_ex (lab (ProgToExecution.G s)).
+
+Lemma dom_rmw_in_rex_add_preserves thread s s'
+      (WF : wf_thread_state thread s) lbl vl lc cl ff
+      (UG : G s' =
+            add (G s) thread (eindex s) lbl vl lc cl ff) 
+      (SS : dom_rmw_in_rex s) :
+    dom_rmw_in_rex s'.
+Proof.
+  unfold dom_rmw_in_rex in *.
+  unfold add in UG. rewrite UG. simpls.
+  rewrite (dom_l (wft_rmwE WF)). rewrite dom_eqv1.
+  rewrite SS.
+  unfold R_ex. unfolder. ins. desc.
+  rewrite updo; auto.
+  intros HH; subst. apply WF.(acts_rep) in H. desf. lia.
+Qed.
+
+Lemma dom_rmw_in_rex_add_rmw_preserves thread s s'
+      (WF : wf_thread_state thread s) lbl1 rexmod ordw vl lc vl' lc' cl ff
+      (UG : G s' =
+            add_rmw (G s) thread (eindex s) (Aload rexmod ordw vl lc)
+                    lbl1 vl' lc' cl ff) 
+      (REX : rexmod = true)
+      (SS : dom_rmw_in_rex s) :
+    dom_rmw_in_rex s'.
+Proof.
+  unfold dom_rmw_in_rex, R_ex in *.
+  unfold add_rmw in UG. rewrite UG. simpls.
+  rewrite dom_union. unionL.
+  2: { rewrite (dom_l (wft_rmwE WF)). rewrite dom_eqv1.
+       unfolder. ins. desc.
+       rewrite !updo; auto.
+       { apply SS. red. eauto. }
+       all: intros HH; subst.
+       all: apply WF.(acts_rep) in H; desf; lia. }
+  unfolder. ins. desc; subst.
+  rewrite updo.
+  { by rewrite upds. }
+  intros HH. inv HH. lia.
+Qed.
+
+Lemma rmw_is_rex_instr_rexmod rmw rexmod xmod ordr ordw reg lexpr s
+      (RMWREX : rmw_is_rex_instrs s.(instrs))
+      (ISTEP :
+         Some
+           (Instr.update rmw rexmod xmod ordr ordw reg
+                         lexpr) = nth_error (instrs s) (pc s)) :
+  rexmod = true.
+Proof.
+  symmetry in ISTEP; apply nth_error_In in ISTEP.
+  apply RMWREX in ISTEP; simpls; desf.
+Qed.
+
+Lemma dom_rmw_in_rex_thread_step thread s s'
+      (RMWREX : rmw_is_rex_instrs s.(instrs))
+      (WF : wf_thread_state thread s)
+      (STEP : step thread s s')
+      (SS : dom_rmw_in_rex s) :
+  dom_rmw_in_rex s'.
+Proof.
+  unfold dom_rmw_in_rex in *.
+  destruct STEP as [ll STEP]. cdes STEP.
+  destruct ISTEP0.
+  1,2: by rewrite UG.
+  1-4: by eapply dom_rmw_in_rex_add_preserves; eauto.
+  all: eapply dom_rmw_in_rex_add_rmw_preserves; eauto.
+  all: rewrite II in ISTEP.
+  all: eapply rmw_is_rex_instr_rexmod; eauto.
+Qed.
+
+End REX.
+
+Section CASREX.
+
+Definition cas_produces_R_ex_instr (i : Instr.t) : Prop :=
+  match i with
+  | Instr.update (Instr.cas _ _) false _ _ _ _ _ => False
+  | _ => True
+  end.
+
+Definition cas_produces_R_ex_instrs (il : list Instr.t) :=
+  forall (i : Instr.t) (IN : In i il), cas_produces_R_ex_instr i.
+
+Lemma cas_produces_R_ex_instr_rexmod old new rexmod xmod ordr ordw reg lexpr s
+      (RMWREX : cas_produces_R_ex_instrs s.(instrs))
+      (ISTEP :
+         Some
+           (Instr.update (Instr.cas old new) rexmod xmod ordr ordw reg
+                         lexpr) = nth_error (instrs s) (pc s)) :
+  rexmod = true.
+Proof.
+  symmetry in ISTEP; apply nth_error_In in ISTEP.
+  apply RMWREX in ISTEP; simpls; desf.
+Qed.
+
+End CASREX.
