src/promiseToImm/RMWPlainStep.v
@@ -499,7 +499,7 @@ Proof.
       all: type_solver. }
     rewrite IdentMap.gss.
     eexists; eexists; eexists; splits; eauto; simpls.
-    { eapply tau_steps_rmw_is_xacq; eauto. }
+    1,2: by erewrite tau_steps_step_same_instrs; eauto.
     { ins. rewrite IdentMap.gso in TID'; auto.
       edestruct (PROM_DISJOINT thread') as [H|]; eauto.
       left. erewrite Memory.remove_o; eauto. desf. }
@@ -1004,7 +1004,7 @@ Proof.
       all: type_solver. }
     rewrite IdentMap.gss.
     eexists; eexists; eexists; splits; eauto; simpls.
-    { eapply tau_steps_rmw_is_xacq; eauto. }
+    1,2: by erewrite tau_steps_step_same_instrs; eauto.
     { ins. eapply PROM_DISJOINT0; eauto.
       rewrite IdentMap.gso in *; eauto.
       rewrite IdentMap.gso in *; eauto. }
